Cleaned `function_prop_minimal_example.v`

theories/approxis/examples/function_prop_minimal_example.v
@@ -2,24 +2,30 @@ From clutch.approxis Require Import approxis map.
 
 Set Default Proof Using "Type*".
 
-Section defs.
+Section motivating_example.
 
   Variable foo : val.
 
   Definition eager_exec : expr :=
     let: "x" := foo #0 in
-    "x".
+    λ: <>, "x".
   
-  Definition lazy_exec : val :=
-    λ: <>, foo #0.
+  Definition lazy_exec : expr :=
+    let: "x" := ref NONE in
+    λ: <>, match: !"x" with
+      | NONE => let: "v" := foo #0 in "x" <- "v";; "v"
+      | SOME "v" => "v"
+    end.
 
   Section proofs.
+    (* a motivating example *)
     Context `{!approxisRGS Σ}.
 
     Variable H : ⊢ refines top foo foo (lrel_int → lrel_int).
 
     Lemma lazy_eager : ⊢ REL eager_exec << lazy_exec : () → lrel_int.
     Proof. rewrite /eager_exec/lazy_exec.
+      rel_alloc_r x as "Hx".
       rel_pures_l; rel_pures_r.
       rel_bind_l (foo _).
       Fail rel_bind_r (foo _).
@@ -27,23 +33,46 @@ Section defs.
         because reducing foo #0 is not the next step on the RHS,
         we're stuck ↯ *)
     Abort.
+    
+  End proofs.
 
-    Section Determinism.
+  (* Hence, the semantic typing assumption is not enough, we need something stronger *)
+End motivating_example.
 
-    (* easy case : determinism *)
 
-    (* TODO move these definition outside of a context containing an instance of
-      approxis, to make them general *)
+Section rules.
+  Context `{!approxisRGS Σ}.
+
+  Fixpoint ForallSep {A} (P : A → iProp Σ) (l : list A) : (iProp Σ) := match l with
+    | [] => True
+    | h :: t => P h ∗ (ForallSep P t)
+  end.
+
+  Fixpoint ForallSep2 {Σ A B} (P : A → B → iProp Σ) (l1 : list A) (l2 : list B) : (iProp Σ) :=
+  match l1, l2 with
+    | [], [] => True
+    | h1 :: t1, h2 :: t2 => P h1 h2 ∗ (ForallSep2 P t1 t2)
+    | _, _ => False
+  end.
+
+  Fixpoint ForallSep3 {Σ A B C} (P : A → B → C → iProp Σ) (l1 : list A) (l2 : list B) (l3 : list C) : (iProp Σ) :=
+  match l1, l2, l3 with
+    | [], [], [] => True
+    | h1 :: t1, h2 :: t2, h3 :: t3 => P h1 h2 h3 ∗ (ForallSep3 P t1 t2 t3)
+    | _, _, _ => False
+  end.
+
+  Section deterministic.
 
     Definition det_val_fun (f : val) (f_sem : Z -> Z) : Prop :=
-      ∀ {Σ : gFunctors} {approxisRGS0 : approxisRGS Σ} (E : coPset)
+      ∀ (E : coPset)
       (K : list (ectxi_language.ectx_item prob_ectxi_lang))
       (n : Z) (e : expr) (A : lrel Σ),
       (refines E (fill K (#(f_sem n))) e A ⊢ refines E (fill K (f #n)) e A) ∧
       (refines E e (fill K (#(f_sem n))) A ⊢ refines E e (fill K (f #n)) A).
 
     Definition det_val_rel (f : val) : Prop :=
-      ∀ {Σ : gFunctors} {approxisRGS0 : approxisRGS Σ} (E : coPset)
+      ∀ (E : coPset)
       (K : list (ectxi_language.ectx_item prob_ectxi_lang))
       (n : Z) (e : expr) (A : lrel Σ), ∃ (m : Z),
       (refines E (fill K (#(m))) e A ⊢ refines E (fill K (f #n)) e A) ∧
@@ -63,31 +92,12 @@ Section defs.
       rewrite /val1; rel_pures_l; rel_pures_r; iApply "H".
     Qed.
 
-    End Determinism.
+  End deterministic.
 
-    Section LocalRef.
-
-    Fixpoint ForallSep {A} (P : A → iProp Σ) (l : list A) : (iProp Σ) := match l with
-      | [] => True
-      | h :: t => P h ∗ (ForallSep P t)
-    end.
-
-    Fixpoint ForallSep2 {Σ A B} (P : A → B → iProp Σ) (l1 : list A) (l2 : list B) : (iProp Σ) :=
-    match l1, l2 with
-      | [], [] => True
-      | h1 :: t1, h2 :: t2 => P h1 h2 ∗ (ForallSep2 P t1 t2)
-      | _, _ => False
-    end.
-
-    Fixpoint ForallSep3 {Σ A B C} (P : A → B → C → iProp Σ) (l1 : list A) (l2 : list B) (l3 : list C) : (iProp Σ) :=
-    match l1, l2, l3 with
-      | [], [], [] => True
-      | h1 :: t1, h2 :: t2, h3 :: t3 => P h1 h2 h3 ∗ (ForallSep3 P t1 t2 t3)
-      | _, _, _ => False
-    end.
+  Section LocalRef.
 
     Definition iterable_local_refs (f : val) (Nref : nat) : Prop :=
-      ∀ {Σ : gFunctors} {approxisRGS0 : approxisRGS Σ} (E : coPset)
+      ∀ (E : coPset)
       (K : list (ectxi_language.ectx_item prob_ectxi_lang))
       (n : Z) (e : expr) (A : lrel Σ), ∃ (v : val),
       ((∀ (ll : list loc) (lv : list val),
@@ -102,8 +112,6 @@ Section defs.
         let: "x" := ref #0 in
         "x" <- !"x" + "v";;
         ! "x".
-
-    Search list (iProp _).
 
     Lemma iterable2 : iterable_local_refs val2 1.
     Proof. rewrite /iterable_local_refs. intros *.
@@ -130,72 +138,31 @@ Section defs.
       - simpl. iFrame.
     Qed.
     
-    End LocalRef.
+  End LocalRef.
 
-    Section RandCouple.
+  Section RandCouple.
+
+    Definition potential_coupling (f : list loc -> val) (n : Z) (v : val) (lιr : list loc) (llrand : list (list nat)) (lN : list nat) : iProp Σ :=
+      ForallSep3 (fun i l n => (i ↪ₛN (n;l))%I) lιr llrand lN ∗
+      ((ForallSep3 (fun i l n => (i ↪ₛN (n;l))%I) lιr llrand lN) -∗
+       (∀ (E' : coPset) (K' : list (ectxi_language.ectx_item prob_ectxi_lang)) (e' : expr) (B : lrel Σ),
+          (refines E' e' (fill K' v) B) -∗ (refines E' e' (fill K' ((f lιr) #n)) B))).
+
+    Definition couplable_rand (f : list loc -> val) (C : lrel Σ) (lN : list nat) : Prop :=
+      ∀ (E : coPset)
+      (K : list (ectxi_language.ectx_item prob_ectxi_lang))
+      (n : Z) (e : list loc -> expr) (A : lrel Σ) (lιl lιr : list loc),
+      (ForallSep2 (fun i n => i ↪N (n;[])) lιl lN ∗ ForallSep2 (fun i n => i ↪ₛN (n;[])) lιr lN ∗
+        ∀ (v : val) (H : ⊢ C v v) (llrand : list (list nat)),
+          potential_coupling f n v lιr llrand lN -∗
+          (refines E (fill K v) (e lιr) A))
+      ⊢ (refines E (fill K (f lιl #n)) (e lιr) A).
     
-    Fixpoint init_tapes (lN : list nat) (e : expr) : expr := match lN with
-      | [] => e
-      | h :: t => let: "_fresh_" := alloc #h in (init_tapes t e) (* change for an actually fresh name *)
-    end.
-
-    Definition potential_coupling := True.
-
     Definition val3 (l : list loc) : val := match l with
       | [ι] => λ: "v", "v" + rand(#lbl:ι) #10
       | _ => λ: <>, #()
     end.
 
-    Definition foo1 : val := λ: <>, rand("i") #10.
-
-    Definition alloc_before_f (f : val) (ι : loc) : expr := prob_lang.subst "i" #lbl:ι f.
-
-    Definition foo2 : expr := let: "i" := alloc #10 in λ: <>, rand("i") #10.
-
-    Lemma test (ι ι' : loc) : ι ↪N (10;[]) ∗ ι' ↪N (10;[])
-      ⊢ refines ⊤ (alloc_before_f foo1 ι) (alloc_before_f foo1 ι') ().
-    Proof. rewrite /alloc_before_f/foo1.
-      rel_pures_l; rel_pures_r. simpl.
-    Abort.
-
-    Lemma test' :
-      ⊢ refines ⊤ foo2 foo2 ().
-    Proof. rewrite /foo2.
-      rel_alloctape_l ι as "Hι". rel_pures_l.
-      rel_alloctape_r ι' as "Hι'". rel_pures_r.
-    Admitted.
-
-    Lemma test'' : ⊢ refines ⊤ (let: "i" := alloc #10 in foo1) (let: "i" := alloc #10 in foo1) ().
-    Proof. rewrite /alloc_before_f/foo1. rel_alloctape_l i as "Hi".
-      rel_alloctape_r i' as "Hi'".
-      rel_pures_l; rel_pures_r.
-    Abort.
-    
-    Definition couplable_rand (f : list loc -> val) (C : lrel Σ) (lN : list nat) : Prop :=
-      ∀ {Σ : gFunctors} {approxisRGS0 : approxisRGS Σ} (E : coPset)
-      (K : list (ectxi_language.ectx_item prob_ectxi_lang))
-      (n : Z) (e : list loc -> expr) (A : lrel Σ) (lιl lιr : list loc),
-      (ForallSep2 (fun i n => i ↪N (n;[])) lιl lN ∗ ForallSep2 (fun i n => i ↪ₛN (n;[])) lιr lN ∗
-        ∀ (v : val) (H : ⊢ C v v) (llrand : list (list nat)),
-          (ForallSep3 (fun i l n => i ↪ₛN (n;l)) lιr llrand lN ∗
-          ((ForallSep3 (fun i l n => i ↪ₛN (n;l)) lιr llrand lN) -∗
-          (∀ (E' : coPset) (K' : list (ectxi_language.ectx_item prob_ectxi_lang))
-            (e' : expr) (B : lrel Σ),
-            (refines E' e' (fill K' v) B) -∗ (refines E' e' (fill K' ((f lιr) #n)) B)))) -∗
-          (refines E (fill K v) (e lιr) A))
-      ⊢ (refines E (fill K (f lιl #n)) (e lιr) A).
-(*
-    Definition couplable_rand_simple (f : expr -> val) (N : nat) : Prop := 
-      ∀ {Σ : gFunctors} {approxisRGS0 : approxisRGS Σ} (E : coPset)
-      (K : list (ectxi_language.ectx_item prob_ectxi_lang))
-      (n : Z) (e : expr -> expr) (e' : expr) (A : lrel Σ) (ι ι' : loc),
-      (ι ↪N (N; []) ∗ ι' ↪ₛN (N; []) ∗
-        ∀ (v : val) (lr : list nat),
-         (ι' ↪ₛN (N; lr) ∗
-          (ι' ↪ₛN (N; lr) -∗ (refines E e' (fill K v) A) -∗ (refines E e' (fill K ((f #lbl:ι') #n)) A))) -∗
-          (refines E (fill K v) (e #lbl:ι') A))
-      ⊢ (refines E (fill K (f #lbl:ι #n)) (e #lbl:ι') A).*)
-    
     Lemma iterable_val3 : couplable_rand val3 lrel_int [10].
     Proof with rel_pures_l; rel_pures_r. rewrite /couplable_rand. intros *.
       iIntros "[Hι [Hι' H]]".
@@ -206,8 +173,6 @@ Section defs.
       destruct lιr as [|hιr tιr]; try destruct tιr as [|hιr' tιr]; simpl;
       try done; try (iDestruct "Hι" as "[_ Hι]"; done); try (iDestruct "Hι'" as "[_ Hι']"; done).
       iDestruct "Hι" as "[Hι _]"; iDestruct "Hι'" as "[Hι' _]".
-
-
       rel_apply (refines_couple_TT_err 10 10); try lia.
       { Unshelve. 6:{ exact 0%R. } 1: { lra. } all: shelve. }
       iFrame.
@@ -223,7 +188,9 @@ Section defs.
       iPureIntro. iStartProof. iExists _. done.
     Qed.
 
-    End RandCouple.
+  End RandCouple.
+
+  Section opaque_example.
 
   Variable foo' : list loc -> val.
   Variable l : list nat.
@@ -249,8 +216,8 @@ Section defs.
     ⊢ REL (eager_exec' li) << lazy_exec'  li' : () → lrel_int.
   Proof with rel_pures_l; rel_pures_r. rewrite /eager_exec'. iIntros "[Hi Hi']".
     rel_bind_l (foo' _ _).
-    iPoseProof (test _ _ ⊤ [AppRCtx (λ: "x" <>, "x")] 0 lazy_exec') as "H". rel_apply "H".
-    iClear "H". iFrame. iIntros (v Hsemtyped llrand) "[Hι' Hiter]".
+    About couplable_rand.
+    iPoseProof (test with "[Hi Hi']") as "H"; last iAssumption. iFrame. iIntros (v Hsemtyped llrand) "[Hι' Hiter]".
     rel_pures_l. rewrite /lazy_exec'.
     rel_alloc_r x as "Hx"...
     set (P := (
@@ -278,9 +245,7 @@ Section defs.
     - rel_apply refines_na_close; iFrame.
       rel_values.
   Qed.
-      
+  
+End opaque_example.
 
-  End proofs.
-
-
-End defs.
+End rules.
